src/threadpool/exec.v
@@ -1,0 +1,134 @@
+From ITree Require Import ITree Eqit Recursion RecursionFacts TranslateFacts.
+From iris.proofmode Require Import proofmode.
+From iris.itree Require Import exec.
+From iris.itree.threadpool Require Import handler.
+
+
+(** * [threadpool] *)
+Program Definition threadpoolEH {GE R} : eHandler threadpoolE GE R :=
+  EHandler (nat * list (option (itree GE R)))
+    (prod_relation (=) (Forall2 (option_Forall2 (eutt eq)))) (λ A e s,
+      match e with
+      | EFork => λ k C, C (k CurrentThread) (s.1, s.2 ++ [Some (k NewThread)])
+      | EYield => λ k C,
+          let tp' := <[s.1 := Some (k tt)]>s.2 in
+          ∃ i t', tp' !! i = Some (Some t') ∧ C t' (i, <[i := None]>tp')
+      | EKillThread => λ k C,
+          (* No need to set s.1 to None since it is already None *)
+          let tp' := s.2 in
+          ∃ i t', tp' !! i = Some (Some t') ∧ C t' (i, <[i := None]>tp')
+      end) _ _ _.
+Next Obligation. move => ???????? Hmono /=. case_match; naive_solver. Qed.
+Next Obligation.
+  move => /= * [tid1 ?] [tid2 ?] [Ht Hs] ?? Hk ?? HC Hh. case_match; simplify_eq/=.
+  - apply: HC; [..|done].
+    + apply: Hk.
+    + constructor; [done|] => /=. apply Forall2_app; [done|].
+      apply Forall2_cons. split; [|done]. constructor. apply Hk.
+  - move: Hh => [i [y' [ ]]].
+    move: (Hs) => /Forall2_length?.
+    move => /list_lookup_insert_Some[[?[??]]|[??]] ?; simplify_eq.
+    + eexists i, _. rewrite list_lookup_insert. 2: lia. split; [done|].
+      apply: HC; [apply Hk|..|done].
+      constructor; [done|] => /=. apply Forall2_insert. 2: by constructor.
+      apply Forall2_insert; [done|]. by constructor.
+    + ogeneralize* Forall2_lookup_l; [done..|] => -[? [? ]]. inv 1.
+      eexists i, _. rewrite list_lookup_insert_ne //. split; [done|].
+      apply: HC; [done|..|done].
+      constructor; [done|] => /=. apply Forall2_insert. 2: by constructor.
+      apply Forall2_insert; [done|]. by constructor.
+  - move: Hh => [i [y' [ ]]].
+    move: (Hs) => /Forall2_length? ??.
+    ogeneralize* Forall2_lookup_l; [done..|] => -[? [? ]]. inv 1.
+    eexists i, _. split; [done|].
+    apply: HC; [done|..|done].
+    constructor; [done|] => /=. apply Forall2_insert. 2: by constructor.
+    done.
+Qed.
+
+Lemma big_sepL2_omap_id_insert {Σ A B} x (l : list (option A)) (Ms : list B) (P : A → B → iProp Σ) i M:
+  l !! i = Some None →
+  ([∗ list] t;M∈omap id l;Ms, P t M) -∗
+  P x M -∗
+  ∃ Ms', ⌜Ms' ≡ₚ M :: Ms⌝ ∗ ([∗ list] t;M∈omap id (<[i:=Some x]>l);Ms', P t M).
+Proof.
+  iIntros (Hi) "Hs Hp".
+  erewrite <-(take_drop_middle l i). 2: done.
+  rewrite omap_app. csimpl.
+  iDestruct (big_sepL2_app_inv_l with "Hs") as (Ms1 Ms2 ?) "[Hs1 Hs2]". subst.
+  iExists (Ms1 ++ M :: Ms2). iSplit.
+  - iPureIntro. by rewrite Permutation_middle.
+  - move: (Hi) => /(lookup_lt_Some _ _ _)?.
+    rewrite insert_app_r_alt take_length_le // ?Nat.sub_diag/= ?omap_app; csimpl.
+    2,3:lia.
+    iApply (big_sepL2_app with "Hs1"). iFrame.
+Qed.
+
+Lemma big_sepL2_omap_id_delete {Σ A B} x (l : list (option A)) (Ms : list B) (P : A → B → iProp Σ) i:
+  l !! i = Some (Some x) →
+  ([∗ list] t;M∈omap id l;Ms, P t M) -∗
+  ∃ M Ms', ⌜Ms ≡ₚ M :: Ms'⌝ ∗ P x M ∗ ([∗ list] t;M∈omap id (<[i:=None]>l);Ms', P t M).
+Proof.
+  iIntros (Hi) "Hs".
+  erewrite <-(take_drop_middle l i). 2: done.
+  rewrite omap_app. csimpl.
+  iDestruct (big_sepL2_app_inv_l with "Hs") as (Ms1 Ms2' ?) "[Hs1 Hs2]".
+  iDestruct (big_sepL2_cons_inv_l with "Hs2") as (M Ms2 ?) "[Hx Hs2]".  subst.
+  iExists M, (Ms1 ++ Ms2). iFrame. iSplit.
+  - iPureIntro. by rewrite Permutation_middle.
+  - move: (Hi) => /(lookup_lt_Some _ _ _)?.
+    rewrite insert_app_r_alt take_length_le // ?Nat.sub_diag/= ?omap_app; csimpl.
+    2,3:lia.
+    iApply (big_sepL2_app with "Hs1"). iFrame.
+Qed.
+
+Global Program Instance threadpoolEH_adequate {Σ GE R} `{!invGS_gen hlc Σ} :
+  eHandlerAdequate (GE:=GE) (R:=R) (threadpoolH) (threadpoolEH) := {|
+    ehandler_inv ts Ms := (⌜ts.2 !! ts.1 = Some None⌝ ∗
+     [∗ list] t;M∈(omap id ts.2);Ms,
+        bi_close (eutt eq) (λ t, ⌜M = λ P, |={⊤,∅}=> P t⌝) t)%I
+  |}.
+Next Obligation.
+  move => ??????? e s Ms C k He.
+  iIntros "HH [% Hs]". rewrite /threadpoolH/=. case_match; simplify_eq/=.
+  - iDestruct "HH" as "[Hc Hn]".
+    iModIntro. iExists _, _, _, _,
+      [λ P, P (k CurrentThread); λ P, |={⊤,∅}=> P (k NewThread)]%I => /=.
+    iSplit; [done|] => /=. iFrame => /=.
+    iSplit; [|iSplitL; [iSplit|]].
+    + iPureIntro. f_equiv. by rewrite Permutation_cons_append.
+    + iPureIntro. rewrite lookup_app_l //. by apply: lookup_lt_Some.
+    + rewrite omap_app /=. iApply big_sepL2_snoc. iFrame. by iApply bi_close_intro.
+    + iApply bi_close_intro. by iIntros (?) "$".
+  - destruct He as (?&?&Hl&?). iMod "HH". iApply fupd_mask_intro; [done|].
+    iDestruct (big_sepL2_omap_id_insert (k ()) with "Hs []") as (? Hperm1) "Hs"; [done|..].
+    { iApply bi_close_intro. done. }
+    iDestruct (big_sepL2_omap_id_delete with "Hs") as (?? Hperm2) "[Hx Hs]"; [done|].
+    iIntros "Hmask". iExists _, _, _, _,
+      [λ P, |={⊤,∅}=> P (k ())]%I => /=.
+    iSplit; [done|] => /=. iFrame => /=.
+    iSplit; [| iSplit].
+    * iPureIntro. by rewrite -Hperm1 Hperm2.
+    * iPureIntro. rewrite list_lookup_insert // insert_length.
+      move: Hl => /(lookup_lt_Some _ _ _). by rewrite insert_length.
+    * iDestruct "Hx" as %(?&->&->). iApply bi_close_intro. iIntros (?) "HP". by iMod "Hmask".
+  - destruct He as (?&?&Hl&?). iMod "HH". iApply fupd_mask_intro; [done|].
+    iDestruct (big_sepL2_omap_id_delete with "Hs") as (???) "[Hx Hs]"; [done|].
+    iIntros "Hmask". iExists _, _, _, _, []%I => /=.
+    iSplit; [done|] => /=. iFrame => /=.
+    iSplit; [| iSplit].
+    * iPureIntro. by rewrite H1.
+    * iPureIntro. rewrite list_lookup_insert //. by apply: lookup_lt_Some.
+    * iDestruct "Hx" as %(?&->&->). iApply bi_close_intro. iIntros (?) "HP". by iMod "Hmask".
+Qed.
+Next Obligation.
+  move => ????? [??] [??] [Htid Hs] ? Ms ->. simplify_eq/=.
+  iIntros "[%Hl HM]". iSplit.
+  - iPureIntro. ogeneralize* Forall2_lookup_l; [done..|].
+    move => [? [? ]]. by inv 1.
+  - clear Hl. iInduction Hs as [|? ? ? ? Ho] "IH" forall (Ms); [done|].
+    inv Ho; csimpl.
+    + iDestruct (big_sepL2_cons_inv_l with "[$]") as (?? ->) "[Hx Hs]" => /=.
+      iSplitL "Hx"; [by rewrite H|]. by iApply "IH".
+    + by iApply "IH".
+Qed.
